spec/extraction/Generic.ec
@@ -4,23 +4,6 @@ from Jasmin require import JModel.
 
 require import Array2 Array3 Array4 Array32 Array64 Array67 Array128 Array2144.
 
-op list_of_array2    ['a] (x : 'a Array2.t)   : 'a list = mkseq (fun (i : int) => x.[i]) 2.
-op list_of_array3    ['a] (x : 'a Array3.t)   : 'a list = mkseq (fun (i : int) => x.[i]) 3.
-op list_of_array4    ['a] (x : 'a Array4.t)   : 'a list = mkseq (fun (i : int) => x.[i]) 4.
-op list_of_array32   ['a] (x : 'a Array32.t)  : 'a list = mkseq (fun (i : int) => x.[i]) 32.
-op list_of_array64   ['a] (x : 'a Array64.t)  : 'a list = mkseq (fun (i : int) => x.[i]) 64.
-op list_of_array67   ['a] (x : 'a Array67.t)  : 'a list = mkseq (fun (i : int) => x.[i]) 67.
-op list_of_array128  ['a] (x : 'a Array128.t) : 'a list = mkseq (fun (i : int) => x.[i]) 128.
-op list_of_array2144 ['a] (x: 'a Array2144.t) : 'a list = mkseq (fun (i :int) => x.[i]) 2144.
-
-op array3_of_list    ['a] (x : 'a list) : 'a Array3.t    = Array3.init    (fun (i : int) => nth witness x i).
-op array4_of_list    ['a] (x : 'a list) : 'a Array4.t    = Array4.init    (fun (i : int) => nth witness x i).
-op array32_of_list   ['a] (x : 'a list) : 'a Array32.t   = Array32.init   (fun (i : int) => nth witness x i).
-op array64_of_list   ['a] (x : 'a list) : 'a Array64.t   = Array64.init   (fun (i : int) => nth witness x i).
-op array67_of_list   ['a] (x : 'a list) : 'a Array67.t   = Array67.init   (fun (i : int) => nth witness x i).
-op array128_of_list  ['a] (x : 'a list) : 'a Array128.t  = Array128.init  (fun (i : int) => nth witness x i).
-op array2144_of_list ['a] (x : 'a list) : 'a Array2144.t = Array2144.init (fun (i : int) => nth witness x i).
-
 module Memcpy = {
   (* This assumes that offset + inlen <= OUTLEN *)
   (* I.e. writing INLEN elements starting at index offset does not write past the end of the array *)
@@ -56,22 +39,20 @@ module Memcpy = {
     return (out, offset);
   }
 
-    proc __memcpy_u8u8_2 (out:W8.t list, out_offset:W64.t,
-                          in_0:W8.t list, in_offset:W64.t,
-                          bytes:W64.t) : W8.t list * W64.t * W64.t = {
+    proc __memcpy_u8u8_2 (out:W8.t list, in_0:W8.t list, in_offset:W64.t,
+                          bytes:W64.t) : W8.t list * W64.t = {
 
     var i:W64.t;
 
     i <- (W64.of_int 0);
 
     while ((i \ult bytes)) {
-      (* out.[(W64.to_uint out_offset)] <- in_0.[(W64.to_uint in_offset)]; *)
-      out <- put out (W64.to_uint out_offset) (nth witness in_0 (W64.to_uint in_offset));
+      (* out.[(W64.to_uint i)] <- in_0.[(W64.to_uint in_offset)]; *)
+      out <- put out (W64.to_uint i) (nth witness in_0 (W64.to_uint in_offset));
       i <- (i + (W64.of_int 1));
       in_offset <- (in_offset + (W64.of_int 1));
-      out_offset <- (out_offset + (W64.of_int 1));
     }
-    return (out, out_offset, in_offset);
+    return (out, in_offset);
   }
 }.
 
