spec/Correctness_Conditions.ec
@@ -1,0 +1,30 @@
+pragma Goals : printall.
+
+require import AllCore List RealExp IntDiv.
+from Jasmin require import JModel.
+require import XMSS_IMPL.
+
+
+(* cond = a < b /\ a < c *)
+lemma cond_u32_a_below_b_and_a_below_c(_a : W32.t, _b : W32.t, _c : W32.t) : 
+    hoare[M(Syscall).__cond_u32_a_below_b_and_a_below_c :
+      arg = (_a, _b, _c) ==> 
+         res = (W32.to_uint _a) < (W32.to_uint _b) /\ (W32.to_uint _a) < (W32.to_uint _c)].
+proof.
+proc.
+auto => />.
+admit.
+qed.
+
+
+(* cond = a >= b /\ c == d *)
+(* cond = b <= a /\ c = d *)
+lemma cond_u64_geq_u64_u32_eq_u32(_a : W64.t, _b : W64.t, _c : W32.t, _d :W32.t) :
+    hoare[M(Syscall).__cond_u64_geq_u64_u32_eq_u32 :
+      arg = (_a, _b, _c, _d) ==>
+        res = (W64.to_uint _b) <= (W64.to_uint _a) /\ (W32.to_uint _c) = (W32.to_uint _d)].
+proof.
+proc.
+auto => />.
+admit.
+qed.
